Fix Diaframe.

theories/zoo/iris/diaframe/symb_exec/wp.v
@@ -1,567 +1,210 @@
-From iris.bi Require Export
-  bi
-  telescopes.
 From iris.proofmode Require Import
-  tactics
-  notation
-  reduction.
+  ltac_tactics.
 
 From diaframe Require Import
   util_classes
-  tele_utils
   solve_defs.
 
+From zoo Require Import
+  prelude.
 From zoo.iris.program_logic Require Import
   wp.
-From zoo.iris.diaframe Require Import
+From zoo.iris.diaframe Require Export
   symb_exec.defs.
+From zoo Require Import
+  options.
 
-Import bi.
-
-(* This file instantiates the symbolic execution interface defined in defs for weakest preconditions *)
-
-Set Universe Polymorphism.
-Lemma to_tforall {TT : tele} (Ψ : TT → Prop) :
-  tforall Ψ → (∀ x, Ψ x).
-Proof.
-  apply tforall_forall.
-Qed.
-Unset Universe Polymorphism.
-
-Ltac drop_telescope_tac tele_name intro_pat :=
-  revert tele_name; refine (to_tforall _ _); intros intro_pat.
-
-Tactic Notation "drop_telescope" constr(R) "as" simple_intropattern_list(intro_pat) :=
-  drop_telescope_tac R intro_pat.
-
-(* useful for pure execution: skips solving a trivial precondition *)
-Definition template_I {PROP : bi} n (M : PROP → PROP) {TT : tele} : (TT → PROP) → PROP
-  := (λ Q, ▷^n (emp -∗ ∀.. (tt : TT), M $ Q tt))%I.
-#[global] Arguments template_I {_} n M {TT} /.
-
-Section template_I_props.
-  Context {PROP : bi}.
-
-  Lemma template_I_strong_mono n TT (M : PROP → PROP) :
-    (∀ P Q, (P -∗ Q) -∗ M P -∗ M Q) →
-    template_strong_mono (template_I n M (TT := TT)).
-  Proof.
-    move => HM P Q /=.
-    iIntros "HPQ HMP !> _" (tt).
-    rewrite left_id bi_tforall_elim.
-    iRevert "HMP". by iApply HM.
-  Qed.
-
-  Lemma template_I_mono TT n (M : PROP → PROP) :
-    ModalityMono M →
-    template_mono (template_I n M (TT := TT)).
-  Proof.
-    move => HM P Q /= HPQ.
-    iIntros "HMP !> _" (tt).
-    rewrite left_id bi_tforall_elim.
-    iApply HM; last done. done.
-  Qed.
-End template_I_props.
-
-Section wp_executor.
+Section iris_G.
   Context `{iris_G : !IrisG Λ Σ}.
 
-  Instance wp_execute_op : ExecuteOp (iPropI Σ) (expr Λ) [tele_pair coPset; val Λ → iPropI Σ] :=
-    λ e, (λᵗ E Φ, WP e @ E {{ Φ }})%I.
-  #[global] Arguments wp_execute_op e !R /.
+  Implicit Types TT : tele.
 
-  #[global] Instance as_wp_execution e E Φ :
-    AsExecutionOf (WP e @ E {{ Φ }})%I wp_execute_op e [tele_arg3 E; Φ].
+  #[global] Instance absorb_modal_fupd_wp e tid E1 E2 Φ :
+    SolveSepSideCondition (E2 ⊆ E1) →
+    AbsorbModal
+      (WP e ∷ tid @ E1 {{ Φ }})
+      (fupd E2 E2)
+      (WP e ∷ tid @ E1 {{ Φ }}).
   Proof.
-    done.
+    rewrite /AbsorbModal. auto.
   Qed.
 
-  Instance wp_red_cond : ReductionCondition (iPropI Σ) (expr Λ) [tele_pair coPset] := (
-    λ A, λᵗ E, λ e e' M,
-      ∀ Φ,
-      M (λ a, WP e' a @ E {{ Φ }}) -∗
-      WP e @ E {{ Φ }}
-  )%I.
-  #[global] Arguments wp_red_cond A !R e e' M /.
-
-  #[global] Instance wp_red_cond_well_behaved_equiv A :
-    Proper (
-      (=) ==> (=) ==>
-      (pointwise_relation _ (=)) ==>
-      ((pointwise_relation _ (⊣⊢)) ==> (⊣⊢)) ==> (⊣⊢)
-    ) (wp_red_cond A).
-  Proof.
-    move => w1 w -> {w1} e1 e -> {e1} e'' e' Hee' M1 M2 HM.
-    drop_telescope w as E => /=.
-    apply (anti_symm _).
-    all: apply forall_mono=> Φ.
-    all: rewrite HM // => a.
-    all: by rewrite Hee'.
-  Qed.
-  #[global] Instance wp_red_cond_well_behaved_ent A :
-    Proper (
-      (=) ==> (=) ==>
-      (pointwise_relation _ (=)) ==>
-      ((pointwise_relation _ (flip (⊢))) ==> (flip (⊢))) ==> (⊢)
-    ) (wp_red_cond A).
-  Proof.
-    move => w1 w -> {w1} e1 e -> {e1} e'' e' Hee' M1 M2 HM.
-    drop_telescope w as E => /=.
-    apply forall_mono=> Φ.
-    apply wand_mono => //.
-    apply HM => a /=.
-    by rewrite Hee'.
-  Qed.
-  #[global] Instance wp_red_cond_well_behaved_tne A :
-    Proper (
-      (=) ==> (=) ==>
-      (pointwise_relation _ (=)) ==>
-      ((pointwise_relation _ (⊢)) ==> (⊢)) ==> (flip (⊢))
-    ) (wp_red_cond A).
-  Proof.
-    move => w1 w -> {w1} e1 e -> {e1} e'' e' Hee' M1 M2 HM.
-    drop_telescope w as E => /=.
-    apply forall_mono=> Φ.
-    apply wand_mono => //.
-    apply HM => a.
-    by rewrite Hee'.
-  Qed.
-
-  Instance language_ctx_condition : ContextCondition (expr Λ) :=
-    λ K,
-      LanguageCtx K.
-
-  #[global] Instance language_ctx_satisfies K :
-    LanguageCtx K →
-    SatisfiesContextCondition language_ctx_condition K.
-  Proof.
-    auto.
-  Qed.
-  #[global] Arguments language_ctx_condition K /.
-
-  Instance wp_template_condition : TemplateCondition (iPropI Σ) [tele_pair coPset; val Λ  → iPropI Σ] :=
-    λ A R M R' M',
-      template_mono M ∧ R = R' ∧ M = M'.
-  #[global] Arguments wp_template_condition _ _ _ /.
-
-  #[global] Instance templateM_satisfies_wp_template_condition R n M1 M2 TT1 TT2 Ps Qs :
-    ModalityMono M1 →
-    ModalityMono M2 →
-    SatisfiesTemplateCondition wp_template_condition R (template_M n M1 M2 TT1 TT2 Ps Qs) R (template_M n M1 M2 TT1 TT2 Ps Qs).
-  Proof.
-    rewrite /SatisfiesTemplateCondition /= => HM1 HM2.
-    split => //.
-    by apply template_M_is_mono.
-  Qed.
-
-  #[global] Instance wp_execute_reduction_compat :
-    ExecuteReductionCompatibility wp_execute_op (λᵗ E _, [tele_arg3 E]) wp_red_cond language_ctx_condition wp_template_condition.
-  Proof.
-    move => K e A e' M /= HK R R' M' [HM [<- <-]].
-    drop_telescope R as E Φ => /=.
-    rewrite -wp_bind'.
-    apply wand_elim_l'.
-    rewrite forall_elim /=.
-    apply wand_mono => //.
-    apply HM => a /=.
-    (* by apply wp_bind_inv. *)
-  Admitted.
-
-  Lemma pure_wp_step_exec `(e : expr Λ) φ n e' E P :
-    Inhabited (state Λ) →
-    PureExec φ n e e' →
-    ReductionStep (wp_red_cond, [tele_arg3 E]) e ⊣ ⟨id⟩ ⌜φ⌝ ; P =[▷^n]=> ⟨id⟩ e' ⊣ emp.
-  Proof.
-    rewrite /ReductionStep' => HS H1 /=.
-    apply forall_intro => Φ.
-    apply wand_intro_l.
-    rewrite -assoc.
-    apply wand_elim_l', pure_elim' => Hφ.
-    apply wand_intro_r.
-    rewrite !left_id (affine P) right_id /=.
-    rewrite -wp_pure_step_later //.
-    apply laterN_mono, wand_mono => //. eauto.
-  Qed.
-
-  Lemma pure_wp_step_exec_lc `(e : expr Λ) φ n e' E P :
-    Inhabited (state Λ) →
-    PureExec φ n e e' →
-    ReductionStep (wp_red_cond, [tele_arg3 E]) e ⊣ ⟨id⟩ ⌜φ⌝ ; P =[▷^n]=> ⟨id⟩ e' ⊣ £ n.
-  Proof.
-    rewrite /ReductionStep' => HS H1 /=.
-    apply forall_intro => Φ.
-    apply wand_intro_l.
-    rewrite -assoc.
-    apply wand_elim_l', pure_elim' => Hφ.
-    apply wand_intro_r.
-    rewrite !left_id (affine P) right_id /=.
-    by rewrite -wp_pure_step_later.
-  Qed.
-
-  Lemma pure_wp_step_exec_lc_fupd `(e : expr Λ) φ n e' E P :
-    Inhabited (state Λ) →
-    PureExec φ n e e' →
-    ReductionStep (wp_red_cond, [tele_arg3 E]) e ⊣ ⟨fupd E E⟩ ⌜φ⌝ ; P =[▷^n]=> ⟨fupd E E⟩ e' ⊣ £ n.
-  Proof.
-    rewrite /ReductionStep' => HS H1 /=.
-    apply forall_intro => Φ.
-    apply wand_intro_l => /=.
-    iIntros "[>H1 H2]"; iStopProof.
-    rewrite -assoc.
-    apply wand_elim_l', pure_elim' => Hφ.
-    apply wand_intro_r.
-    rewrite !left_id (affine P) right_id /=.
-    rewrite -wp_pure_step_later //.
-    apply bi.laterN_mono.
-    apply bi.wand_mono; first done.
-    by iMod 1.
-  Qed.
-
-  Lemma pure_wp_step_exec2 `(e : expr Λ) φ n e' E P :
-    Inhabited (state Λ) →
-    PureExec φ n e e' →
-    SolveSepSideCondition φ →
-    ReductionTemplateStep wp_red_cond [tele] P [tele_arg3 E] e (tele_app (TT := [tele]) e') (template_I n (fupd E E)).
-  Proof.
-    rewrite /ReductionTemplateStep /SolveSepSideCondition => HS H1 Hφ /=.
-    apply forall_intro => Φ.
-    apply wand_intro_l.
-    rewrite (affine P) right_id.
-    rewrite -wp_pure_step_later //.
-    apply bi.laterN_mono, wand_mono, fupd_wp. eauto.
-  Qed.
-
-  #[global] Instance later_forall_satisfies_template_condition n R (TT : tele) M :
-    ModalityMono M →
-    SatisfiesTemplateCondition wp_template_condition R (template_I n M (TT := TT)) R (template_I n M).
-  Proof.
-    rewrite /SatisfiesTemplateCondition /=.
-    split => //. by apply template_I_mono.
-  Qed.
-
-  Lemma as_unit_fun_texan P e v Q E :
-    {{{ P }}} e @ E {{{ RET v; Q }}} →
-    {{{ P }}} e @ E {{{ (_ : ()), RET v; Q }}}.
-  Proof.
-    move => HT Φ.
-    iIntros "HP HΦ". iApply (HT with "HP").
-    iIntros "!> HQ". by iApply ("HΦ" $! tt).
-  Qed.
-
-  Lemma later_if_laterN_if {PROP : bi} (P : PROP) (p : bool) :
-    ▷^ (if p then 1 else 0) P ⊣⊢@{PROP} ▷?p P.
-  Proof.
-    done.
-  Qed.
-
-  Lemma later_if_sep {PROP : bi} (P Q : PROP) (p : bool) :
-    ▷?p (P ∗ Q) ⊣⊢@{PROP} ▷?p P ∗ ▷?p Q.
-  Proof.
-    case: p => //=. apply later_sep.
-  Qed.
-
-  Lemma if_bool_as_nat (n : nat) (p : bool) :
-    TCOr (TCAnd (TCEq n 1) (TCEq p true)) (TCAnd (TCEq n 0) (TCEq p false)) →
-    n = if p then 1 else 0.
-  Proof.
-    by case => [[-> ->] | [-> ->]].
-  Qed.
-
-  (* this is basically sym-ex-fupd-exist, but stated in terms of ReductionStep' *)
-  Lemma texan_to_red_cond (A B : tele) n p P e Q (f : A -t> B -t> val Λ) f' E1 E2 :
-    TCOr (TCAnd (TCEq n 1) (TCEq p true)) (TCAnd (TCEq n 0) (TCEq p false)) →
-    (∀.. (a : A) (b : B), tele_app (tele_app f' a) b = of_val (tele_app (tele_app f a) b)) →
-    TCOr (Atomic e) (TCEq E1 E2) →
-    (* the following rule reduces to texan triple notation when B is a constructor. *)
-    (∀.. a : A, ∀ Φ,
-      tele_app P a -∗ ▷ (∀.. (b : B), tele_app (tele_app Q a) b -∗ Φ (tele_app (tele_app f a) b)) -∗ WP e @ E2 {{ Φ }}) →
-    ReductionStep' wp_red_cond (ε₀)%I n (fupd E1 E2) (fupd E2 E1) A B P Q e f' [tele_arg3 E1].
-  Proof.
-    rewrite /ReductionStep' => /if_bool_as_nat ->
-      /tforall_forall Hf' HeE /tforall_forall HT.
-    apply forall_intro => Φ.
-    apply wand_intro_r.
-    rewrite empty_hyp_first_eq left_id /=.
-    match goal with
-    | |- (fupd ?E1 ?E2 ?Hp ⊢ WP ?e @ E1 {{ ?Φ }}) =>
-      enough (Hp ⊢ WP e @ E2 {{ fupd E2 E1 ∘ Φ }})
-    end.
-    - destruct HeE as [He | <-].
-      * rewrite -wp_atomic.
-        by apply fupd_mono.
-      * rewrite -fupd_wp -wp_fupd.
-        by apply fupd_mono.
-    - apply bi_texist_elim => a.
-      rewrite later_if_laterN_if.
-      wlog:p /(p = true) => [ | -> /=].
-      { case: p; [ move => H; by apply H | (move => <-; last done) => /=; by rewrite -bi.later_intro ]. }
-      iIntros "[HP HΦ]". iApply (HT with "HP").
-      iStopProof. apply later_mono, bi_tforall_mono => b.
-      apply wand_mono; first done => /=.
-      specialize (Hf' a); apply to_tforall with _ b in Hf'; rewrite Hf' => /=.
-      erewrite wp_value_fupd => //. rewrite fupd_trans //.
-  Qed.
-
-  (* here is a slightly more readable version: *)
-  Lemma sym_ex_fupd_exist (A B : tele) P e Q (f : A -t> B -t> val Λ) E1 E2 K `{LanguageCtx Λ K} Ψ :
-    Atomic e ∨ (E1 = E2) →
-    (* the following rule reduces to texan triple notation when B is a constructor. *)
-    (∀.. a : A, ∀ Φ,
-      tele_app P a -∗ ▷ (∀.. (b : B), tele_app (tele_app Q a) b -∗ Φ (tele_app (tele_app f a) b)) -∗ WP e @ E2 {{ Φ }}) →
-    (|={E1,E2}=> ∃.. (a : A), tele_app P a ∗ ▷ (∀.. (b : B), tele_app (tele_app Q a) b -∗ |={E2, E1}=> WP (K $ of_val (tele_app (tele_app f a) b)) @ E1 {{ Ψ }}))
-      ⊢ WP (K e) @ E1 {{ Ψ }}.
-  Proof.
-    move => Hmask He.
-    rewrite -(wp_bind _ _ None None) //.
-    match goal with
-    | |- (fupd ?E1 ?E2 ?Hp ⊢ WP ?e @ E1 {{ ?Φ }}) =>
-      enough (Hp ⊢ WP e @ E2 {{ fupd E2 E1 ∘ Φ }})
-    end.
-    - destruct Hmask as [Hat | <-].
-      * rewrite -wp_atomic.
-        by apply fupd_mono.
-      * rewrite -fupd_wp -wp_fupd.
-        by apply fupd_mono.
-    - apply bi_texist_elim => a.
-      revert He => /(dep_eval_tele a) HT.
-      iIntros "[HP HΦ]". by iApply (HT with "HP").
-  Qed.
-
-  #[global] Instance reduction_step_from e E Φ :
-    ReductionStep (wp_red_cond, [tele_arg3 E]) e ⊣ ⟨fupd E E⟩ emp; WP e @ E {{ Φ }} =[▷^0]=> ∃ v, ⟨fupd E E⟩ of_val v ⊣ Φ v.
-  Proof.
-    rewrite /ReductionStep' /ReductionTemplateStep /=.
-    apply forall_intro => Ψ.
-    apply wand_intro_l.
-    eapply entails_po; [ | apply wand_elim_l'; by iApply wp_strong_mono ].
-    rewrite sep_comm.
-    apply sep_mono_r.
-    apply forall_intro => v.
-    rewrite (forall_elim v) => /=.
-    erewrite wp_value_fupd => //. rewrite !left_id fupd_trans.
-    iIntros "HΦΨ HΦ".
-    by iMod ("HΦΨ" with "HΦ") as "H".
-  Qed.
-
-  Lemma iris_goal_to_red_cond (A B : tele) n P e Q f' E1 E2 pre (POST : (val Λ → iProp Σ) → A -t> B -t> iProp Σ) :
-    TCOr (TCAnd (Atomic e) $
-                (∃ fv, ∀.. (a : A), ∀.. (b : B), (AsVal (tele_app (tele_app f' a) b) (tele_app (tele_app fv a) b)))
-      )
-      (TCEq E1 E2) →
-    (∃ fv, (∀.. (a : A), ∀.. (b : B), (AsVal (tele_app (tele_app f' a) b) (tele_app (tele_app fv a) b))) ∧
-          (TCEq POST (λ Φ, tele_map (tele_map Φ) fv))) ∨
-          (TCEq POST (λ Φ, tele_map (tele_map (λ fe, WP fe @ E2 {{ Φ }}))%I f')) →
-    (* the following rule reduces to texan triple notation when B is a constructor. *)
-    (∀.. a : A, ∀ Φ,
-      pre ∗ tele_app P a -∗ ▷^n (∀.. (b : B), tele_app (tele_app Q a) b -∗ (tele_app (tele_app (POST Φ) a) b)) -∗ WP e @ E2 {{ Φ }}) →
-    ReductionStep' wp_red_cond pre n (fupd E1 E2) (fupd E2 E1) A B P Q e f' [tele_arg3 E1].
-  Proof.
-    rewrite /ReductionStep' => HeE HPOST /tforall_forall HT.
-    apply forall_intro => Φ.
-    apply wand_intro_r => /=.
-    rewrite fupd_frame_l.
-    match goal with
-    | |- (fupd ?E1 ?E2 ?Hp ⊢ WP ?e @ E1 {{ ?Φ }}) =>
-      enough (Hp ⊢ WP e @ E2 {{ fupd E2 E1 ∘ Φ }})
-    end.
-    - destruct HeE as [[He1 _] | <-].
-      * rewrite -wp_atomic.
-        by apply fupd_mono.
-      * rewrite -fupd_wp -wp_fupd.
-        by apply fupd_mono.
-    - apply wand_elim_r', bi_texist_elim => a.
-      apply wand_intro_l. rewrite assoc.
-      iIntros "[HP HΦ]". iApply (HT with "HP").
-      iStopProof.
-      apply laterN_mono, bi_tforall_mono => b.
-      apply wand_mono => //.
-      destruct HeE as [[_ He2] | <-]; last first.
-      * rewrite fupd_wp.
-        destruct HPOST as [[fv [Hf ->]] | ->].
-        + rewrite !tele_map_app /=.
-          revert Hf => /(dep_eval_tele a) /(dep_eval_tele b) <-.
-          rewrite wp_value_fupd' //.
-        + rewrite !tele_map_app /=.
-          apply wp_mono => //= v.
-          exact: fupd_intro.
-      * destruct HPOST as [[fv' [Hf ->]] | ->].
-        + revert Hf => /(dep_eval_tele a) /(dep_eval_tele b) <-.
-          rewrite !wp_value_fupd' /= fupd_trans !tele_map_app //=.
-        + rewrite !tele_map_app /=.
-          case: He2 => fv /(dep_eval_tele a) /(dep_eval_tele b) <-.
-          rewrite !wp_value_fupd' => /=.
-          rewrite fupd_trans.
-          exact: fupd_intro.
-  Qed.
-
-  #[global] Instance red_cond_emp_valid_atomic_no_Φ (A B : tele) P e Q f' fv w E1 E2 pre :
-    TCEq (tele_app (TT := [tele_pair coPset]) (λ E, E) w) E1 →
-    Atomic e →
-    TCEq (to_val e) None →
-    (∀.. (a : A), ∀.. (b : B), (AsVal (tele_app (tele_app f' a) b) (tele_app (tele_app fv a) b))) →
-    (* the following rule reduces to texan triple notation when B is a constructor. *)
-    AsEmpValidWeak
-      (ReductionStep' wp_red_cond pre 1 (fupd E1 E2) (fupd E2 E1) A B P Q e f' w)
-      ((∀.. a : A,
-      pre ∗ tele_app P a -∗ WP e @ E2 {{ λ v, ∃.. (b : B), ⌜v = tele_app (tele_app fv a) b⌝ ∗ tele_app (tele_app Q a) b }})) | 10.
-  Proof.
-    drop_telescope w as E' => /= ->.
-    rewrite /AsEmpValidWeak.
-    move => He1 He2 Hfv HPQ.
-    eapply iris_goal_to_red_cond.
-    - left. split => //. exists fv. done.
-    - left. exists fv. done.
-    - apply tforall_forall => a Φ /=.
-      iIntros "Hpre Hlater".
-      iApply (wp_step_fupd with "[Hlater]"); first done.
-      { iIntros "!> !>". iApply "Hlater". } iStopProof.
-      revert HPQ.
-      rewrite bi_tforall_forall.
-      rewrite (bi.forall_elim a) => /wand_entails ->.
-      apply wp_mono => v /=.
-      iIntros "[%b [-> HQ]] HΦ".
-      iSpecialize ("HΦ" $! b).
-      rewrite !tele_map_app.
-      by iApply "HΦ".
-  Qed.
-
-  #[global] Instance red_cond_emp_valid_value (A B : tele) n P e Q f' fv E1 pre w :
-    TCEq (tele_app (TT := [tele_pair coPset]) (λ E, E) w) E1 →
-    (∀.. (a : A), ∀.. (b : B), (AsVal (tele_app (tele_app f' a) b) (tele_app (tele_app fv a) b))) →
-    (* the following rule reduces to texan triple notation when B is a constructor. *)
-    AsEmpValidWeak
-      (ReductionStep' wp_red_cond pre n (fupd E1 E1) (fupd E1 E1) A B P Q e f' w)
-      ((∀.. a : A, ∀ Φ,
-      pre ∗ tele_app P a -∗ ▷^n (∀.. (b : B), tele_app (tele_app Q a) b -∗ Φ (tele_app (tele_app fv a) b)) -∗ WP e @ E1 {{ Φ }})) | 50.
-  Proof.
-    drop_telescope w as E' => /= ->.
-    rewrite /AsEmpValidWeak.
-    move => Hfv HPQ.
-    eapply iris_goal_to_red_cond.
-    - tc_solve.
-    - left. exists fv. done.
-    - apply tforall_forall => a Φ.
-      revert HPQ.
-      rewrite bi_tforall_forall.
-      rewrite (bi.forall_elim a).
-      rewrite (bi.forall_elim Φ) => /wand_entails ->.
-      iIntros "HWP HΦ". iApply "HWP". iStopProof.
-      by do 2 setoid_rewrite tele_map_app.
-  Qed.
-
-  Lemma red_cond_emp_valid_value_no_Φ (A B : tele) P e Q f' fv E1 pre :
-    (∀.. (a : A), ∀.. (b : B), (AsVal (tele_app (tele_app f' a) b) (tele_app (tele_app fv a) b))) →
-    (* the following rule reduces to texan triple notation when B is a constructor. *)
-    AsEmpValidWeak
-      (ReductionStep' wp_red_cond pre 0 (fupd E1 E1) (fupd E1 E1) A B P Q e f' [tele_arg3 E1])
-      ((∀.. a : A,
-      pre ∗ tele_app P a -∗ WP e @ E1 {{ λ v, ∃.. (b : B), ⌜v = tele_app (tele_app fv a) b⌝ ∗ tele_app (tele_app Q a) b }})).
-  Proof. (* so.. the texan version is stronger, since it allows us to eliminate laters? *)
-    rewrite /AsEmpValidWeak.
-    move => Hfv HPQ.
-    eapply iris_goal_to_red_cond.
-    - tc_solve.
-    - left. exists fv. done.
-    - apply tforall_forall => a Φ.
-      revert HPQ.
-      rewrite bi_tforall_forall.
-      rewrite (bi.forall_elim a).
-      move => /wand_entails -> /=.
-      iIntros "HWP HΦ". iApply (wp_wand with "HWP").
-      iIntros (v) "[%b [-> HQ]]".
-      iSpecialize ("HΦ" with "HQ"). by rewrite !tele_map_app.
-  Qed.
-
-  #[global] Instance red_cond_emp_valid_value_no_Φ_not_value (A B : tele) P e Q f' fv E1 pre w :
-    TCEq (tele_app (TT := [tele_pair coPset]) (λ E, E) w) E1 →
-    TCEq (to_val e) None →
-    (∀.. (a : A), ∀.. (b : B), (AsVal (tele_app (tele_app f' a) b) (tele_app (tele_app fv a) b))) →
-    (* the following rule reduces to texan triple notation when B is a constructor. *)
-    AsEmpValidWeak
-      (ReductionStep' wp_red_cond pre 1 (fupd E1 E1) (fupd E1 E1) A B P Q e f' w)
-      ((∀.. a : A,
-      pre ∗ tele_app P a -∗ WP e @ E1 {{ λ v, ∃.. (b : B), ⌜v = tele_app (tele_app fv a) b⌝ ∗ tele_app (tele_app Q a) b }})) | 20.
-  Proof. (* so.. the texan version is stronger, since it allows us to eliminate laters? *)
-    drop_telescope w as E' => /= ->.
-    rewrite /AsEmpValidWeak.
-    move => He Hfv HPQ.
-    eapply iris_goal_to_red_cond.
-    - tc_solve.
-    - left. exists fv. done.
-    - apply tforall_forall => a Φ /=.
-      iIntros "Hpre Hlater".
-      iApply (wp_step_fupd with "[Hlater]"); first done.
-      { iIntros "!> !>". iApply "Hlater". } iStopProof.
-      revert HPQ.
-      rewrite bi_tforall_forall.
-      rewrite (bi.forall_elim a).
-      move => /wand_entails ->.
-      iApply wp_mono => v /=.
-      iIntros "[%b [-> HQ]] HΦ".
-      iSpecialize ("HΦ" $! b).
-      rewrite !tele_map_app.
-      by iApply "HΦ".
-  Qed.
-
-  #[global] Instance red_cond_emp_valid_not_value (A B : tele) n P e Q f' E1 pre w :
-    TCEq (tele_app (TT := [tele_pair coPset]) (λ E, E) w) E1 →
-    AsEmpValidWeak
-      (ReductionStep' wp_red_cond pre n (fupd E1 E1) (fupd E1 E1) A B P Q e f' w)
-      ((∀.. a : A, ∀ Φ,
-      pre ∗ tele_app P a -∗ ▷^n (∀.. (b : B), tele_app (tele_app Q a) b -∗ WP (tele_app (tele_app f' a) b) @ E1 {{ Φ }}) -∗ WP e @ E1 {{ Φ }})) | 25.
-  Proof.
-    drop_telescope w as E' => /= ->.
-    rewrite /AsEmpValidWeak.
-    move => HPQ.
-    eapply iris_goal_to_red_cond.
-    - tc_solve.
-    - right. tc_solve.
-    - apply tforall_forall => a Φ.
-      revert HPQ.
-      rewrite bi_tforall_forall.
-      rewrite (bi.forall_elim a).
-      rewrite (bi.forall_elim Φ) => /wand_entails ->.
-      do 2 setoid_rewrite tele_map_app.
-      by iIntros "$".
-  Qed.
-End wp_executor.
-
-(* this instance makes iSteps work on goals built by Program, which for some reason unfolds ReductionStep' goals *)
-#[global] Instance template_step_emp_valid {PROP : bi} (pre : PROP) `(red_cond : ReductionCondition PROP E W) e n M1 M2 (A B : tele) P' f'  Q w G :
-  AsEmpValidWeak (PROP := PROP) (ReductionStep' red_cond pre n M1 M2 A B P' Q e f' w) G →
-  AsEmpValidWeak (PROP := PROP) (ReductionTemplateStep red_cond (qprod A B) pre w e
-    (λ pr, tele_app (tele_app f' $ qfst pr) $ qsnd pr) (template_M (PROP := PROP) n M1 M2 A B P' Q)) G.
-Proof.
-  done.
-Qed.
-
-Section abducts.
-  Context `{iris_G : !IrisG Λ Σ}.
-
-  #[global] Instance abduct_from_execution P Q e R K e_in' T e_out' MT MT' R' :
-    AsExecutionOf P wp_execute_op e R →
-    ReshapeExprAnd (expr Λ) e K e_in' (ReductionTemplateStep wp_red_cond T Q%I ((λᵗ E _, [tele_arg3 E]) R) e_in' e_out' MT) →
-    SatisfiesContextCondition language_ctx_condition K →
-    SatisfiesTemplateCondition wp_template_condition R MT R' MT' →
-    HINT1 Q ✱ [MT' $ flip wp_execute_op R' ∘ K ∘ e_out'] ⊫ [id]; P.
-  Proof.
-    intros. eapply execution_abduct_lem => //. tc_solve.
-  Qed.
-
-  #[global] Instance collect_modal_wp_value e v E Φ :
+  #[global] Instance dia_wp_value e v E Φ :
     AsVal e v →
-    HINT1 ε₀ ✱ [fupd E E $ Φ v] ⊫ [id]; WP e @ E {{ Φ }} | 10.
+    HINT1 ε₀ ✱ [
+      |={E}=> Φ v
+    ] ⊫ [id];
+      WP e @ E {{ Φ }}
+  | 10.
   Proof.
     rewrite /AsVal /Abduct /= empty_hyp_first_eq left_id => <-.
     erewrite wp_value_fupd => //.
   Qed.
 
-  #[global] Instance prepend_modal_wp_expr e E Φ :
-    PrependModality (WP e @ E {{ Φ }})%I (fupd E E) (WP e @ E {{ Φ }})%I | 20.
+  #[global] Instance dia_wp_mono e1 K e2 e2' tid E Φ1 Φ2 :
+    ReshapeExprAnd _ e1 K e2' (TCEq e2' e2) →
+    LanguageCtx K →
+    HINT1
+      WP e2 ∷ tid @ E {{ Φ2 }}
+    ✱ [
+      ∀ v2,
+      Φ2 v2 -∗
+      WP K (of_val v2) ∷ tid @ E {{ Φ1 }}
+    ] ⊫ [id];
+      WP e1 ∷ tid @ E {{ Φ1 }}.
   Proof.
-    rewrite /PrependModality.
-    apply (anti_symm _).
-    - rewrite -{2}fupd_wp //.
-    - apply fupd_intro.
+    iIntros ((-> & ->) HK) "(HΦ2 & HΦ1)".
+    iApply wp_bind'.
+    iApply (wp_wand with "HΦ2"). iIntros "%v2 HΦ2".
+    iApply ("HΦ1" with "HΦ2").
   Qed.
-End abducts.
+
+  Class DiaSpec TT1 TT2 P e E ret Q :=
+    dia_spec Φ :
+      ∀.. tt1 : TT1,
+      tele_app P tt1 -∗
+      ▷ (
+        ∀.. tt2 : TT2,
+        tele_app (tele_app Q tt1) tt2 -∗
+        Φ (tele_app (tele_app ret tt1) tt2)
+      ) -∗
+      WP e @ E {{ Φ }}.
+  #[global] Arguments dia_spec _ _ _ _ _ _ _ {_} _ : assert.
+
+  #[global] Instance dia_spec_as_emp_valid_weak TT1 TT2 P e E ret Q :
+    AsEmpValidWeak
+      (DiaSpec TT1 TT2 P e E ret Q)
+      ( ∀ Φ,
+        ∀.. tt1 : TT1,
+        tele_app P tt1 -∗
+        ▷ (
+          ∀.. tt2 : TT2,
+          tele_app (tele_app Q tt1) tt2 -∗
+          Φ (tele_app (tele_app ret tt1) tt2)
+        ) -∗
+        WP e @ E {{ Φ }}
+      ).
+  Proof.
+    rewrite /DiaSpec. iIntros "%". done.
+  Qed.
+
+  #[global] Instance dia_wp_spec e K e' TT1 TT2 P ret Q tid E1 E2 Φ :
+    ReshapeExprAnd _ e K e' (
+      TCOr (
+        TCAnd
+          (Atomic e')
+          (DiaSpec TT1 TT2 P e' E2 ret Q)
+      ) (
+        TCAnd
+          (TCEq E1 E2)
+          (DiaSpec TT1 TT2 P e' E1 ret Q)
+      )
+    ) →
+    LanguageCtx K →
+    HINT1 ε₀ ✱ [
+      |={E1,E2}=>
+      ∃.. tt1,
+      tele_app P tt1 ∗
+      ▷ ∀.. tt2,
+        tele_app (tele_app Q tt1) tt2 ={E2,E1}=∗
+        WP K $ of_val $ tele_app (tele_app ret tt1) tt2 ∷ tid @ E1 {{ Φ }}
+    ] ⊫ [id];
+      WP e ∷ tid @ E1 {{ Φ }}.
+  Proof.
+    rewrite /Abduct /=.
+    iIntros ((-> & Hspec) HK) "(_ & H)".
+    iApply wp_bind'.
+    iApply wp_thread_id_mono.
+    destruct Hspec as [(Hatomic & Hspec) | (<- & Hspec)].
+    all: iMod "H" as "(%tt1 & HP & H)".
+    all: iApply (Hspec with "HP").
+    all: iIntros "!> %tt2 HQ".
+    all: iMod ("H" with "HQ") as "H".
+    all: iApply "H".
+  Qed.
+End iris_G.
+
+Declare Custom Entry dia_spec_mask.
+Notation "" := (
+  @top coPset _
+)(in custom dia_spec_mask
+).
+Notation "@ E" :=
+  E
+( in custom dia_spec_mask at level 200,
+  E constr,
+  format "'/  ' @  E "
+).
+
+Notation "'DIASPEC' {{ P } } e E {{ 'RET' v ; Q } }" := (
+  DiaSpec
+    TeleO
+    TeleO
+    P%I
+    e%E
+    E
+    v%V
+    Q%I
+)(at level 20,
+  P at level 200,
+  e at level 200,
+  E custom dia_spec_mask at level 200,
+  Q at level 200,
+  format "'[hv' DIASPEC  {{  '/  ' '[' P ']'  '/' } }  '/  ' '[' e ']'  E '/' {{  '/  ' RET  v ;  '/  ' '[' Q ']'  '/' } } ']'"
+) : stdpp_scope.
+Notation "'DIASPEC' x1 .. xn {{ P } } e E {{ 'RET' v ; Q } }" := (
+  DiaSpec
+    (TeleS (λ x1, .. (TeleS (λ xn, TeleO)) ..))
+    TeleO
+    (λ x1, .. (λ xn, P%I) ..)
+    e%E
+    E
+    (λ x1, .. (λ xn, v%V) ..)
+    (λ x1, .. (λ xn, Q%I) ..)
+)(at level 20,
+  x1 binder,
+  xn binder,
+  P at level 200,
+  e at level 200,
+  E custom dia_spec_mask at level 200,
+  Q at level 200,
+  format "'[hv' DIASPEC  x1  ..  xn  {{  '/  ' '[' P ']'  '/' } }  '/  ' '[' e ']'  E '/' {{  '/  ' RET  v ;  '/  ' '[' Q ']'  '/' } } ']'"
+) : stdpp_scope.
+Notation "'DIASPEC' {{ P } } e E {{ y1 .. yn , 'RET' v ; Q } }" := (
+  DiaSpec
+    TeleO
+    (TeleS (λ y1, .. (TeleS (λ yn, TeleO)) ..))
+    P%I
+    e%E
+    E
+    (λ y1, .. (λ yn, v%V) ..)
+    (λ y1, .. (λ yn, Q%I) ..)
+)(at level 20,
+  P at level 200,
+  e at level 200,
+  E custom dia_spec_mask at level 200,
+  y1 binder,
+  yn binder,
+  Q at level 200,
+  format "'[hv' DIASPEC  {{  '/  ' '[' P ']'  '/' } }  '/  ' '[' e ']'  E '/' {{  y1  ..  yn ,  '/  ' RET  v ;  '/  ' '[' Q ']'  '/' } } ']'"
+) : stdpp_scope.
+Notation "'DIASPEC' x1 .. xn {{ P } } e E {{ y1 .. yn , 'RET' v ; Q } }" := (
+  DiaSpec
+    (TeleS (λ x1, .. (TeleS (λ xn, TeleO)) ..))
+    (TeleS (λ y1, .. (TeleS (λ yn, TeleO)) ..))
+    (λ x1, .. (λ xn, P%I) ..)
+    e%E
+    E
+    (λ x1, .. (λ xn, λ y1, .. (λ yn, v%V) ..) ..)
+    (λ x1, .. (λ xn, λ y1, .. (λ yn, Q%I) ..) ..)
+)(at level 20,
+  x1 binder,
+  xn binder,
+  P at level 200,
+  e at level 200,
+  E custom dia_spec_mask at level 200,
+  y1 binder,
+  yn binder,
+  Q at level 200,
+  format "'[hv' DIASPEC  x1  ..  xn  {{  '/  ' '[' P ']'  '/' } }  '/  ' '[' e ']'  E '/' {{  y1  ..  yn ,  '/  ' RET  v ;  '/  ' '[' Q ']'  '/' } } ']'"
+) : stdpp_scope.
